lean/privacy/channels/channels.lean
@@ -13,8 +13,10 @@ def channel_exists (crypto: Crypto) (m: Memory) (c: ℕ) : Prop :=
 -- CreateChannel action → Kbob has a corresponding private key.
 theorem exists_private_key
     {crypto: Crypto} {inp: CreateChannelInput} {rm: ReachableMemory crypto}
-    (success: (create_channel crypto inp rm |> process_action crypto rm).2) :
-    ∃ kbob ∈ crypto.PrivateKeys, inp.Kbob = crypto.priv_to_pub kbob := by
+    (success: (create_channel crypto inp rm |> process_action crypto rm).success) :
+    ∃ kbob: crypto.PrivateKeys,
+      inp.Kbob = crypto.priv_to_pub kbob ∧
+      rm.m .PrivateKeyHashes [inp.addrbob, kbob] = 1 := by
   let info := create_channel_info crypto inp rm success
   have bob_registered := info.bob_registered
   rw [←info.h_Kbob] at bob_registered
@@ -28,8 +30,14 @@ theorem channel_exists_implies_hash
     {crypto: Crypto} {c addralice addrbob Kbob: ℕ} :
     ∀ {rm: ReachableMemory crypto},
     rm.m .ChannelHashes [crypto.hash [c, addralice, addrbob, Kbob]] ≠ 0 →
-    ∃ kalice, c = crypto.hash [addralice, kalice, addrbob, Kbob] ∧
-    ∃ kbob: crypto.PrivateKeys, Kbob = crypto.priv_to_pub kbob := by
+    (∃ kalice,
+      c = crypto.hash [addralice, kalice, addrbob, Kbob] ∧
+      rm.m .PrivateKeyHashes [addralice, kalice] ≠ 0
+    ) ∧
+    (∃ kbob: crypto.PrivateKeys,
+      Kbob = crypto.priv_to_pub kbob ∧
+      rm.m .PrivateKeyHashes [addrbob, kbob] = 1
+    ) := by
   apply ReachableMemory.induction
   case inv₀ => intro h; trivial
 
@@ -37,23 +45,101 @@ theorem channel_exists_implies_hash
   cases action
   case CreateChannel inp =>
     let info := create_channel_info crypto inp rm success
-    dsimp only [ReachableMemory.add, run_action]
-    rw [←info.h_m']
+    dsimp only [ReachableMemory.add, ReachableMemory.m]
+    rw [run_all_cons₁, run_action, ←info.h_m']
     intro h'
 
     by_cases h_is_same: c = inp.c crypto ∧ addralice = inp.addralice ∧ addrbob = inp.addrbob ∧ Kbob = inp.Kbob
     case pos =>
-      simp [h_is_same]
+      simp only [h_is_same]
       constructor
       · use inp.kalice
-      · exact exists_private_key success
+        constructor
+        · trivial
+        · rw [info.no_change _ _ (by simp)]
+          exact info.kalice_valid
+      · conv => rhs; intro kbob; rw [info.no_change _ _ (by simp)]
+        have := exists_private_key success
+        exact exists_private_key success
     case neg =>
-      rw [info.no_change _ _ (by simp) (by simp) (by
-        simp only [ne_eq, Prod.mk.injEq, List.cons.injEq, and_true, true_and]
+      rw [info.no_change _ _  (by
+        simp only [ne_eq, Prod.mk.injEq, reduceCtorEq, List.cons.injEq, List.ne_cons_self,
+          and_false, and_self, not_false_eq_true, List.nil_eq, and_true, true_and]
         by_contra h'
         apply crypto.h_hash at h'
         repeat injection h' with _ h'
         simp [*] at h_is_same
       )] at h'
+      conv => rhs; rhs; intro m'; rw [info.no_change _ _ (by simp)]
+      conv => lhs; rhs; intro m'; rw [info.no_change _ _ (by simp)]
       exact ih h'
+
+  case Register inp =>
+    intro h
+    let info := register_info crypto inp rm success
+    rw [rm.add_m, run_action, ←info.h_m']
+
+    have ⟨⟨kalice, h₀, h₁⟩, ⟨kbob, h₂, h₃⟩⟩ := ih h
+    refine ⟨⟨kalice, h₀, ?_⟩, ⟨kbob, h₂, ?_⟩⟩
+    · by_cases h_is_same: addralice = inp.addralice ∧ kalice = inp.kalice
+      case pos => simp [h_is_same, info.memory_diff₁]
+      case neg => rwa [info.no_change _ _ (by simp) (by simp [h_is_same])]
+    · by_cases h_is_same: addrbob = inp.addralice ∧ kbob = inp.kalice
+      case pos => simp only [h_is_same, info.memory_diff₁]
+      case neg => rwa [info.no_change _ _ (by simp) (by simp [h_is_same])]
+
   all_goals exact ih
+
+theorem channel_exists_iff_CreateChannel {crypto: Crypto} {rm: ReachableMemory crypto} {c: ℕ} :
+    channel_exists crypto rm c ↔
+    (∃ inp: CreateChannelInput, .CreateChannel inp ∈ rm.actions ∧ inp.c crypto = c) := by
+  revert rm
+  apply ReachableMemory.induction
+  case inv₀ =>
+    constructor
+    · intro h
+      have ⟨addralice, addrbob, Kbob, h⟩ := h
+      simp [ReachableMemory.m] at h
+    · intro h; simp at h
+
+  intro action rm ih success
+  cases action
+  case CreateChannel inp' =>
+    let info := create_channel_info crypto inp' rm success
+    rw [ReachableMemory.add_m, run_action, ←info.h_m']
+    simp only [channel_exists]
+
+    by_cases h_is_same: c = inp'.c crypto
+    case pos =>
+      constructor
+      · intro h
+        obtain ⟨addralice, addrbob, Kbob, h⟩ := h
+        exact ⟨inp', by simp [ReachableMemory.add], by simp [h_is_same]⟩
+      · intro h
+        use inp'.addralice, inp'.addrbob, inp'.Kbob
+        simp [h_is_same, info.memory_diff₂]
+    case neg =>
+      conv in _ ≠ 0 => rw [info.no_change _ _ (by
+        have : crypto.hash [c, addralice, addrbob, Kbob] ≠ inp'.channel_hash crypto := by
+          by_contra h'; apply crypto.h_hash at h'; injections; contradiction
+        simp [this]
+      )]
+      rw [ReachableMemory.add]
+
+      conv in _ ∈ _ => rw [List.mem_cons, Action.CreateChannel.injEq]
+      rw [←channel_exists, ih]
+
+      constructor
+      · intro h
+        have ⟨inp, h₀, h₁⟩ := h
+        exact ⟨inp, Or.inr h₀, h₁⟩
+      · intro h
+        obtain ⟨inp, h₀, h₁⟩ := h
+        cases h₀
+        case inl h₀ =>
+          rw [←h₁, h₀] at h_is_same
+          contradiction
+        case inr h₀ =>
+          exact ⟨inp, h₀, h₁⟩
+
+  all_goals simpa [ReachableMemory.add]
