lean/privacy/channels/contiguous.lean
@@ -5,24 +5,24 @@ import privacy.channels.channels
 -- Once a channel exists, it stays this way.
 theorem channel_exists_monotone (crypto: Crypto) (rm: ReachableMemory crypto) (action: Action)
   (c: ℕ)
-  (success: (run_action crypto action rm.m).2)
+  (success: (run_action crypto action rm.m).success)
   (h : channel_exists crypto rm c)
   : let rm' := rm.add action success
     channel_exists crypto rm' c
 := by
-  unfold channel_exists ReachableMemory.add run_action
+  unfold channel_exists
   cases action
   case CreateChannel inp =>
     simp only
     let info := create_channel_info crypto inp rm success
     obtain ⟨addralice, addrbob, Kbob, h⟩ := h
     use addralice, addrbob, Kbob
-    rw [←info.h_m']
+    rw [ReachableMemory.add_m, run_action, ←info.h_m']
     by_cases h₀ : crypto.hash [c, addralice, addrbob, Kbob] = inp.channel_hash crypto
     case pos =>
       simp [h₀, info.memory_diff₂]
     case neg =>
-      rwa [info.no_change _ _ (by simp) (by simp) (by simp [h₀])]
+      rwa [info.no_change _ _ (by simp [h₀])]
   all_goals exact h
 
 -- The j-s of the channels for (addrbob, Kbob) form a contiguous range [0, j_bound) where j_bound
@@ -31,17 +31,15 @@ theorem channels_contiguous {crypto: Crypto} (rm: ReachableMemory crypto) (addrb
     ∀ j, (j ≥ rm.m .ChannelsJ [addrbob, Kbob]) ↔ rm.m .Channels [addrbob, Kbob, j] = 0 := by
   revert rm
   apply ReachableMemory.induction
-  case inv₀ => intros; simp
+  case inv₀ => intros; simp [ReachableMemory.m]
 
   intro action rm
   cases action
   case CreateChannel inp =>
     intro h success j
-    unfold ReachableMemory.add run_action
-    dsimp only
 
     have info := create_channel_info crypto inp rm success
-    rw [←info.h_m']
+    rw [ReachableMemory.add_m, run_action, ←info.h_m']
 
     by_cases h_bob: addrbob = inp.addrbob ∧ Kbob = inp.Kbob
     case pos =>
@@ -59,14 +57,84 @@ theorem channels_contiguous {crypto: Crypto} (rm: ReachableMemory crypto) (addrb
         rw [this]
         exact crypto.enc_is_not_zero _ _
       case neg =>
-        rw [info.no_change _ _ (by simp) (by simp [h_j]) (by simp)]
+        rw [info.no_change _ _ (by simp [h_j])]
         constructor
         · intro h₀; rw [h.1 (by omega)]
         · intro h₀
           have := h.2 h₀
           omega
     case neg =>
-        rw [info.no_change _ _ (by simp [h_bob]) (by simp) (by simp)]
-        rw [info.no_change _ _ (by simp) (by by_contra; injections; injections; simp [*] at h_bob) (by simp)]
+        rw [info.no_change _ _ (by simp [h_bob])]
+        rw [info.no_change _ _ (by
+          simp only [ne_eq, Prod.mk.injEq, true_and, List.cons.injEq, List.cons_ne_self, and_false,
+            and_true, reduceCtorEq, not_false_eq_true]
+          by_contra
+          simp [*] at h_bob
+        )]
         exact h j
   all_goals intro h success; exact h
+
+-- The s of outgoing channels for given (addralice, kalice) form a contiguous range [0, s_bound).
+theorem outgoing_channels_contiguous {crypto: Crypto} (rm: ReachableMemory crypto) (addralice kalice: ℕ) :
+    ∃ s_bound, ∀ s, s < s_bound ↔ rm.m .OutgoingChannels [crypto.hash [addralice, kalice, s], 0] ≠ 0 := by
+  revert rm
+  apply ReachableMemory.induction
+  case inv₀ => use 0; intros; simp [ReachableMemory.m]
+
+  intro action rm ih success
+  cases action
+  case CreateChannel inp =>
+    obtain ⟨s_bound, ih⟩ := ih
+    let info := create_channel_info crypto inp rm success
+    rw [ReachableMemory.add_m, run_action, ←info.h_m']
+
+    by_cases h₀ : addralice = inp.addralice ∧ kalice = inp.kalice
+    case pos =>
+      use s_bound + 1
+      intro s
+
+      have h_inp_s_not_small : ¬inp.s < s_bound := by
+        have := (ih inp.s).1
+        simp [h₀, info.outgoing_channel_didnt_exist] at this
+        omega
+
+      have h_inp_s_not_big : ¬inp.s > s_bound := by
+        cases info.prev_outgoing_exists
+        case inl h_prev => omega
+        case inr h_prev =>
+          have := (ih (inp.s - 1)).2
+          simp only [h₀, CreateChannelInput.prev_outgoing_channel_id] at h_prev this
+          omega
+
+      have h_s : s_bound = inp.s := by omega
+
+      by_cases h₁ : s = inp.s
+      case pos =>
+        simp only [h₁, h_s, h₀.1, h₀.2, info.memory_diff₃, lt_add_iff_pos_right, Nat.lt_one_iff,
+          ne_eq, true_iff]
+        exact info.r_ne_zero
+      case neg =>
+        have h_hash_ne : crypto.hash [inp.addralice, inp.kalice, s] ≠ inp.outgoing_channel_id crypto := by
+          simp only [CreateChannelInput.outgoing_channel_id, ne_eq]
+          intro h
+          apply crypto.h_hash at h
+          injections h
+          contradiction
+        rw [h₀.1, h₀.2, info.no_change _ _ (by simp [h_hash_ne])]
+        have := ih s
+        simp only [h₀] at this
+        rw [←this]
+        omega
+    case neg =>
+      use s_bound
+      intro s
+      have h_hash_ne : crypto.hash [addralice, kalice, s] ≠ inp.outgoing_channel_id crypto := by
+        simp only [CreateChannelInput.outgoing_channel_id, ne_eq]
+        intro h
+        apply crypto.h_hash at h
+        injections h
+        omega
+      rw [info.no_change _ _ (by simp [h_hash_ne])]
+      exact ih s
+
+  all_goals exact ih
