lean/privacy/registration/discoverable.lean
@@ -1,0 +1,80 @@
+import privacy.actions
+
+def scan_users (crypto: Crypto) (events: List Event) : List (ℕ × ℕ) :=
+  events |>.filterMap (λ e ↦ match e with
+    | .Register addralice kalice_enc => some (addralice, (crypto.dec crypto.council_priv_key kalice_enc).headD 0)
+  )
+
+theorem scan_users' {crypto: Crypto} {events: List Event} {addralice kalice: ℕ} :
+    (addralice, kalice) ∈ scan_users crypto events ↔
+    (∃ kalice_enc,
+      .Register addralice kalice_enc ∈ events ∧
+      (crypto.dec crypto.council_priv_key kalice_enc).headD 0 = kalice
+    ) := by
+  constructor
+  · intro h
+    rw [scan_users, List.mem_filterMap] at h
+    have ⟨e, h₀, h₁⟩ := h
+    cases e
+    case Register addralice' kalice_enc =>
+      simp only [Option.some.injEq, Prod.mk.injEq] at h₁
+      rw [←h₁.1]
+      exact ⟨kalice_enc, h₀, h₁.2⟩
+  · intro ⟨kalice_enc, h₀, h₁⟩
+    rw [scan_users, List.mem_filterMap]
+    use .Register addralice kalice_enc, h₀
+    simp only [h₁]
+
+theorem scan_users_private_key {crypto: Crypto} (rm: ReachableMemory crypto) {addralice kalice: ℕ}
+    (h: (addralice, kalice) ∈ scan_users crypto rm.events) :
+    kalice ∈ crypto.PrivateKeys := by
+  replace ⟨kalice_enc, h, h₁⟩ := scan_users'.1 h
+
+  revert rm
+  apply ReachableMemory.induction
+  case inv₀ => intro h; contradiction
+
+  intro action rm ih success h
+
+  rw [rm.add_events, List.mem_append] at h
+  cases h
+  case inl h => exact ih h
+  case inr h =>
+    cases action
+    case Register inp =>
+      let info := register_info crypto inp rm success
+      rw [run_action, info.events, List.mem_singleton] at h
+      simp only [Event.Register.injEq] at h
+      convert info.kalice_private_key
+      rw [h.2, crypto.h_council_priv_key, crypto.dec_enc, List.headD_cons] at h₁
+      simp [h₁]
+
+    all_goals contradiction
+
+theorem register_implies_scan_users
+    {crypto: Crypto} {rm: ReachableMemory crypto} {inp: RegisterInput}
+    (h: .Register inp ∈ rm.actions) :
+    (inp.addralice, inp.kalice) ∈ scan_users crypto rm.events := by
+  rw [scan_users']
+
+  revert rm
+  apply ReachableMemory.induction
+  case inv₀ => intro h; contradiction
+
+  intro action rm ih success h
+  rw [rm.add_events]
+  rw [ReachableMemory.add] at h
+  cases h
+  case tail h =>
+    have ⟨kalice_enc, h₀, h₁⟩ := ih h
+    use kalice_enc
+    rw [List.mem_append]
+    exact ⟨Or.inl h₀, h₁⟩
+  case head =>
+    let info := register_info crypto inp rm success
+    use crypto.enc crypto.council_pub_key [inp.kalice]
+    constructor
+    · rw [List.mem_append]
+      apply Or.inr
+      rw [run_action, info.events, List.mem_singleton, crypto.h_council_priv_key]
+    · rw [crypto.h_council_priv_key, crypto.dec_enc, List.headD_cons]
