lean/privacy/registration/registration.lean
@@ -1,0 +1,60 @@
+import privacy.actions
+import privacy.utils
+
+-- If a PublicKeys memory cell is non-zero, then it is a valid public key (private key exists).
+theorem public_keys {crypto: Crypto} {addralice: ℕ} :
+    ∀ {rm: ReachableMemory crypto},
+    rm.m .PublicKeys [addralice] ≠ 0 →
+    ∃ kalice: crypto.PrivateKeys,
+      rm.m .PublicKeys [addralice] = crypto.priv_to_pub kalice ∧
+      rm.m .PrivateKeyHashes [addralice, kalice] = 1 := by
+  apply ReachableMemory.induction
+  case inv₀ => simp [ReachableMemory.m]
+
+  intro action rm
+  cases action
+  case Register inp =>
+    intro h success
+    let info := register_info crypto inp rm success
+    rw [ReachableMemory.add_m, run_action, ←info.h_m']
+
+    by_cases h_addralice: addralice = inp.addralice
+    case pos =>
+      rw [h_addralice, info.memory_diff₀]
+      intro h
+      refine ⟨⟨inp.kalice, info.kalice_private_key⟩, by rfl, info.memory_diff₁⟩
+    case neg =>
+      rw [info.no_change _ _ (by simp [h_addralice]) (by simp)]
+      intro h_public_key_ne_zero
+      conv => rhs; intro kalice; rw [info.no_change _ _ (by simp) (by simp [h_addralice])]
+      exact h h_public_key_ne_zero
+  repeat intro h success; exact h
+
+theorem private_key_hash_implies {crypto: Crypto} {rm: ReachableMemory crypto} {addralice kalice: ℕ}
+    (h: rm.m .PrivateKeyHashes [addralice, kalice] ≠ 0) :
+    ∃ inp: RegisterInput,
+      .Register inp ∈ rm.actions ∧
+      inp.addralice = addralice ∧
+      inp.kalice = kalice := by
+  revert rm
+  apply ReachableMemory.induction
+  case inv₀ => simp [ReachableMemory.m]
+
+  intro action rm ih success h
+  cases action
+  case Register inp =>
+    by_cases h_is_same: addralice = inp.addralice ∧ kalice = inp.kalice
+    case pos =>
+      use inp
+      simp [h_is_same]
+    case neg =>
+      let info := register_info crypto inp rm success
+
+      rw [rm.add_m, run_action, ←info.h_m'] at h
+      rw [info.no_change _ _ (by simp) (by simp [h_is_same])] at h
+      have ⟨inp, h₀, h₁⟩ := ih h
+      exact ⟨inp, by simp [ReachableMemory.add, h₀], h₁⟩
+
+  all_goals
+    have ⟨inp, h₀, h₁⟩ := ih h
+    exact ⟨inp, by simp [ReachableMemory.add, h₀], h₁⟩
