lean/privacy/tracking/coin.lean
@@ -1,0 +1,129 @@
+import privacy.transactions.transactions
+
+abbrev Transaction.ActionIdx (tx: Transaction) := Fin (tx.actions.length)
+
+-- Map from action to optional (token, amount) pair.
+private abbrev CollectCoinsFunc := Action → Option (ℕ × ℕ)
+
+def Transaction.collect_coins (tx: Transaction) (f: CollectCoinsFunc) (token: ℕ) : List (tx.ActionIdx × ℕ) :=
+  tx.actions
+  |>.mapFinIdx (λ idx action h_idx ↦ ((⟨idx, h_idx⟩: tx.ActionIdx), action))
+  |>.flatMap (λ (idx, action) ↦ (
+    f action
+    |>.filter (λ (token', _) ↦ token' = token)
+    |>.map (λ (_, amount) ↦ (List.range amount).map (λ x ↦ (idx, x)))
+    |>.getD []
+  ))
+
+theorem Transaction.collect_coins_length {tx: Transaction} {f: CollectCoinsFunc} {token: ℕ} :
+    (tx.collect_coins f token).length =
+    (tx.actions
+      |>.filterMap f
+      |>.filter (λ (token', _) ↦ token' = token)
+      |>.map (λ (_, amount) ↦ amount) |>.sum) := by
+  unfold Transaction.collect_coins
+  rw [List.length_flatMap]
+  rw [List.map_congr_left (by
+    intro ⟨idx, action⟩ h_idx_action
+    let g := λ a: tx.ActionIdx × Action ↦ (f a.2).map (λ val ↦ if val.1= token then val.2 else 0) |>.getD 0
+    show _ = g (idx, action)
+    simp only [g]
+    cases f action
+    case none => simp
+    case some val =>
+      simp [Option.filter_some]
+      by_cases h: val.1 = token
+      case pos => simp [h]
+      case neg => simp [h]
+  )]
+  rw [map_maxFinIdx]
+  rw [mapFinIdx_eq_map (λ action: Action ↦ (f action).map (λ val ↦ if val.1 = token then val.2 else 0) |>.getD 0)]
+  simp [filter_map_sum_to_ite, filterMap_map_sum_to_getD]
+
+theorem Transaction.collect_coins_nodup {tx: Transaction} {f: CollectCoinsFunc} {token: ℕ} :
+    (tx.collect_coins f token).Nodup := by
+  apply mapFinIdx_flatMap_Nodup (j := λ (idx, x) ↦ idx)
+  case g_nodup =>
+    intro ⟨idx, action⟩
+    simp only
+    cases f action
+    case some val =>
+      by_cases h: val.1 = token
+      case pos =>
+        simp [Option.filter_some, h]
+        apply List.Nodup.map
+        · intro a b hab
+          simp only [Prod.mk.injEq] at hab
+          exact hab.2
+        · exact List.nodup_range
+      case neg => simp [Option.filter_some, h]
+    case none => simp
+
+  case h_j =>
+    intro i action h_idx res h_res
+    simp only at h_res
+    cases h_f: f action
+    case some val =>
+      rw [h_f] at h_res
+      by_cases h: val.1 = token
+      case pos =>
+        simp only [Option.filter_some, h, decide_true, ↓reduceIte, Option.map_some,
+          Option.getD_some, List.mem_map, List.mem_range] at h_res
+        have ⟨_, _, h_res⟩ := h_res
+        rw [←h_res]
+      case neg => simp [Option.filter_some, h] at h_res
+    case none => simp [h_f] at h_res
+
+def Transaction.created_coins (tx: Transaction) (token: ℕ) : List (tx.ActionIdx × ℕ) :=
+  tx.collect_coins
+    (λ action ↦ (filter_CreateNote action).map (λ inp ↦ (inp.token, inp.amount)))
+    token
+
+def Transaction.canceled_coins (tx: Transaction) (token: ℕ) : List (tx.ActionIdx × ℕ) :=
+  tx.collect_coins
+   (λ action ↦ (filter_CancelNote action).map (λ inp ↦ (inp.token, inp.amount)))
+   token
+
+theorem created_coins_length (tx: Transaction) (token: ℕ) :
+    (tx.created_coins token).length = tx.sum_create_note_amounts token := by
+  unfold Transaction.created_coins
+  rw [tx.collect_coins_length]
+  simp only [Transaction₀.sum_create_note_amounts]
+  unfold Transaction₀.sum_amounts ActionFunc.create ActionFuncRes.from_create
+  simp only [List.filter_filterMap, List.map_filterMap]
+  apply congrArg
+  apply List.filterMap_congr
+  intro action h_actions
+  cases action
+  case CreateNote inp =>
+    by_cases h: inp.token = token
+    all_goals simp [h, Option.filter_some]
+
+  all_goals simp
+
+theorem canceled_coins_length (tx: Transaction) (token: ℕ) :
+    (tx.canceled_coins token).length = tx.sum_cancel_note_amounts token := by
+  unfold Transaction.canceled_coins
+  rw [tx.collect_coins_length]
+  simp only [Transaction₀.sum_cancel_note_amounts]
+  unfold Transaction₀.sum_amounts ActionFunc.cancel ActionFuncRes.from_cancel
+  simp only [List.filter_filterMap, List.map_filterMap]
+  apply congrArg
+  apply List.filterMap_congr
+  intro action h_actions
+  cases action
+  case CancelNote inp =>
+    by_cases h: inp.token = token
+    all_goals simp [h, Option.filter_some]
+
+  all_goals simp
+
+-- A bijection between `created_coins.toFinset` and `canceled_coins.toFinset`.
+def Transaction.coins_equiv (tx: Transaction) (token: ℕ) :
+    (tx.created_coins token).toFinset ≃ (tx.canceled_coins token).toFinset :=
+  two_lists_equiv
+    (tx.created_coins token)
+    (tx.canceled_coins token)
+    (by rw [created_coins_length, canceled_coins_length, tx.h_balance])
+    collect_coins_nodup
+    collect_coins_nodup
