lean/privacy/tracking/outgoing_notes.lean
@@ -1,0 +1,121 @@
+import privacy.actions
+import privacy.amounts
+import privacy.compliance.all_notes
+import privacy.notes.canceled_notes
+import privacy.registration.discoverable
+import privacy.transactions.transactions
+import privacy.tracking.utils
+
+theorem outgoing_notes₀
+    {crypto: Crypto} (stxs: SuccessfulTransactions crypto)
+    (addralice: ℕ) (token: ℕ) :
+    (
+      create_note_actions crypto stxs.rm
+      |>.filter (λ inp ↦ inp.token = token ∧ inp.addralice = addralice)
+      |>.map (λ inp ↦ inp.amount)
+      |>.sum
+    ) = (
+      stxs.txs
+      |>.filter (λ tx ↦ tx.owner = addralice)
+      |>.map (λ tx ↦ tx.sum_create_note_amounts token)
+      |>.sum
+    ) := by
+  rw [←filtered_note_actions_to_tx_actions]
+  unfold create_note_actions ActionFunc.create ActionFuncRes.from_create
+  simp only [List.filter_filterMap, List.map_filterMap]
+  apply congrArg
+  apply List.filterMap_congr
+  intro action h_action
+  cases h_some: filter_CreateNote action
+  case none => simp
+  case some inp => simp [Option.filter_some]
+
+theorem outgoing_notes₁
+    {crypto: Crypto} (stxs: SuccessfulTransactions crypto)
+    (addralice: ℕ) (token: ℕ) :
+    let kalices : List ℕ :=
+      scan_users crypto stxs.rm.events
+      |>.filter (λ user ↦ user.1 = addralice)
+      |>.map (λ user ↦ user.2)
+      |>.dedup
+    (
+      create_note_actions crypto stxs.rm
+      |>.filter (λ inp ↦ inp.token = token ∧ inp.addralice = addralice)
+      |>.map (λ inp ↦ inp.amount)
+      |>.sum
+    ) =
+    (
+      kalices
+      |>.map (λ kalice ↦
+        create_note_actions crypto stxs.rm
+        |>.filter (λ inp ↦ inp.token = token ∧ inp.addralice = addralice ∧ inp.kalice = kalice)
+        |>.map (λ inp ↦ inp.amount)
+        |>.sum
+      )
+      |>.sum
+    ) := by
+  intro kalices
+  rw [fiber_sum
+    (img:=kalices)
+    (f:=λ inp ↦ inp.kalice)
+    (h_img := by
+      intro inp h_inp
+      rw [List.mem_filter] at h_inp
+      simp only [kalices, List.mem_dedup, List.mem_map, List.mem_filter]
+      use ⟨inp.addralice, inp.kalice⟩
+      refine ⟨⟨?_, ?_⟩, by rfl⟩
+      . have h_exists := create_note_actions_implies h_inp.1
+        have ⟨sn, _, h_sn_note_id, ⟨addralice, kalice, addrbob, kbob, h_c, h_in_scan_users_alice, h_in_scan_users_bob⟩⟩ := all_notes_are_discoverable h_exists.1
+        have : inp.c crypto = sn.c := by
+          apply crypto.h_hash at h_sn_note_id
+          injections
+        have : inp.addralice = addralice ∧ inp.kalice = kalice := by
+          rw [h_c] at this
+          apply crypto.h_hash at this
+          injections
+          rename_i h_kalice _
+          simp [*]
+        simp [this, h_in_scan_users_alice]
+      · simp only [Bool.decide_and, Bool.and_eq_true, decide_eq_true_eq] at h_inp
+        simp [h_inp]
+    )
+    (h_nodup:=by apply List.nodup_dedup)
+  ]
+
+  simp only [←List.filterMap_eq_map, ←List.filterMap_eq_filter, List.filterMap_filterMap]
+  apply congrArg
+  apply List.filterMap_congr
+  intro kalice h_kalice
+  simp only [Function.comp_apply, Option.some.injEq, Option.guard]
+  apply congrArg
+  apply List.filterMap_congr
+  intro inp h_inp
+  by_cases h: inp.token = token ∧ inp.addralice = addralice
+  case pos =>
+    by_cases h': inp.kalice = kalice
+    case pos => simp [h, h']
+    case neg => simp [decide_eq_true h, h']
+  case neg => simp [←and_assoc, h]
+
+theorem outgoing_notes
+    {crypto: Crypto} (stxs: SuccessfulTransactions crypto)
+    (addralice: ℕ) (token: ℕ) :
+    (
+      scan_users crypto stxs.rm.events
+      |>.filter (λ user ↦ user.1 = addralice)
+      |>.map (λ user ↦ user.2)
+      |>.dedup
+      |>.map (λ kalice ↦
+        create_note_actions crypto stxs.rm
+          |>.filter (λ inp ↦ inp.token = token ∧ inp.addralice = addralice ∧ inp.kalice = kalice)
+          |>.map (λ inp ↦ inp.amount)
+          |>.sum
+      )
+      |>.sum
+    )= (
+      stxs.txs
+      |>.filter (λ tx ↦ tx.owner = addralice)
+      |>.map (λ tx ↦ tx.sum_create_note_amounts token)
+      |>.sum
+    ) := by
+  rw [←outgoing_notes₀, ←outgoing_notes₁]
